<!--
@import "/dissertation/assets/custom.md"
 -->
\begin{center}
  \input{assets/amplitude_3pointsimple2.tex}
\end{center}

Vertex, using a cyclic rotation:
$$
\begin{aligned}
  iV_{\mu_1, \mu_2, \mu_3}^{a_1, a_2, a_3} &= ig \left [
    (p_1-p_2)_{\mu_3} \eta_{\mu_1 \mu_2} +
    (p_2-p_3)_{\mu_1} \eta_{\mu_2 \mu_3} +
    (p_3-p_1)_{\mu_2} \eta_{\mu_3 \mu_1}
  \right ]f^{a_1 a_2 a_3}\\
  &=f^{a_1 a_2 a_3} V_{\mu_1 \mu_2 \mu_3}
\end{aligned}
$$

Amplitude, using the polarisation vector $\epsilon_{\alpha\dot{\alpha}}$:
$$
\left .
\begin{aligned}
  V_{
    \mu_1 \mu_2 \mu_3
    } = \evaluated{
      \epsilon_{(1)}^{\mu_1} \epsilon_{(2)}^{\mu_2} \epsilon_{(3)}^{\mu_3}
      }_{
        p_1^2 = p_2^2 = p_3^2 = 0
      }
= &\left [ \left( p_1 - p_2 \right) \cdot \epsilon_{(3)}\right ] \left( \epsilon_{(1)} \cdot \epsilon_{(2)} \right) +\\
  &\left [ \left( p_2 - p_3 \right) \cdot \epsilon_{(1)}\right ] \left( \epsilon_{(2)} \cdot \epsilon_{(3)} \right) +\\
  & \left [ \left( p_3 - p_1 \right) \cdot \epsilon_{(2)}\right ] \left( \epsilon_{(3)} \cdot \epsilon_{(1)} \right)
\end{aligned}
\qquad \right \}
[A]
$$

*   Using this method, we will always have momentum conservation such that $p_1 + p_2 + p_3 = 0$
*   Momentum is always transverse to polarisation $p\cdot \epsilon(p) = 0$

Transverse:
$$
  \epsilon(p) \approx \frac{
    \ld{\alpha}\tilde{\eta}_{\dot{\alpha}}
    }{ \sqr{\lambda}{\eta}
  }  = 0
$$

Simplifying $[A]$:
$$
\begin{aligned}
  -p_2 &= p_1 + p_3\\
  &= (2p_1 +p_3)\cdot \epsilon_3\\
  &= 2(p_1 \cdot \epsilon_3)
\end{aligned}
$$
Likewise, the remaining $p_i$ can be found by cyclicly permutation.

\begin{definition}[Polarisation Vector, reference spinor]
$$
\begin{aligned}
  \epsilon^{+}_{\alpha\dot{\alpha}} & \equiv  \frac{\xi_{\alpha} \tilde{k}_{\dot{\alpha}}}{\agl{\xi}{k}} \sqrt{2}\\
  \epsilon^{-}_{\alpha\dot{\alpha}} & \equiv - \frac{\tilde{\xi}_{\dot{\alpha}} k_{\alpha}}{\sqr{\tilde{\xi}}{\tilde{k}}}\sqrt{2}\\
\end{aligned}
$$
\end{definition}

We use this definition to simplify the following case:

$$
\begin{aligned}
  \tensor{{\epsilon_1}}{_{\alpha\dot{\alpha}}} \cdot \tensor{{\epsilon_2}}{^{\alpha\dot{\alpha}}} &= 2(\epsilon_1\cdot \epsilon_2)\\
  &= \left( - \sqrt{2} \right)^2 \frac{1_{\dot{\alpha}} k_{\alpha}}{ \agl{1}{k} } \frac{2^{\dot{\alpha}} k^\alpha}{ \agl{2}{k}}\\
  &= \sqr{1}{2} \agl{k}{k} = 0
\end{aligned}
$$

Now here we illustrate the case for MHV (Maximum Helicity Violation), where we are choosing as many as possible combinations that can be reduced to 0 on inspection without further need to calculation:
$$
\begin{aligned}
  A(1,2,3) = 2 \left [ (p_i \cdot \epsilon^3)(\epsilon^1 \cdot \epsilon^2) +
  (p_2 \cdot \epsilon^1)(\epsilon^2 \cdot \epsilon^3)
  (p_3 \cdot \epsilon^1)(\epsilon^1 \cdot \epsilon^3)
  \right ]
\end{aligned}
$$

Using

$$
\begin{aligned}
  \epsilon_1^- &= \frac{\tilde{\xi}_{\dot{\alpha}} 1_{\alpha} }{ \sqr{\xi}{1}}\\
  \epsilon_2^- &= \frac{\tilde{\xi}_{\dot{\alpha}} 2_{\alpha} }{ \sqr{\xi}{2}}\\
\end{aligned}
$$

We are now looking for $\epsilon_1^{1^-} \cdot \epsilon_2^{2^-}$

Deriving gluon three-point amplitudes from Feynman rules, colour order:

$$
\begin{aligned}
  2 \cdot \epsilon_2 \epsilon_3 &= \tensor{{\epsilon_{(2)}}}{^{\dot{\alpha}\alpha}} \tensor{{\epsilon_{(3)}}}{_{\alpha \alpha}}\\
  &= \sqrt{2}\sqrt{2} \ 2^{\dot{\alpha}} \underbrace{\tensor{{k_3}}{_{\dot{\alpha}}} \tensor{{k_2}}{^{\alpha}} \tensor{3}{_{\alpha}}}_{Contraction}\\
  &= -2\sqr{k_3}{2} \agl{k_2}{3}
\end{aligned}
$$

Using the definition of the reference spinor

Aiming to find $\perp \therefore a \cdot  b = 0$, which gets rid of the interaction $\Yup$. This makes the first and third term vanish:
$$
  \epsilon_1 \cdot \epsilon_2 = 0, \qquad \epsilon_1 \cdot \epsilon_3 = 0
$$
Leaving us only with the second term:
$$
\begin{aligned}
  \left[
  p_2 \epsilon_1^-
  \right] \left(
    \epsilon_2^- \cdot \epsilon_3^+
  \right) &=
  \tensor{ {p_2} }{_{\alpha\dot{\alpha}}} \left( -\sqrt{2} \right) \frac{
    \tilde{\xi}^{\dot{\alpha}} 1^{\alpha}
    }{
      \tensor{{\lambda_2}}{_{\dot{\alpha}}}
    } \\
  2(p_2 \cdot \epsilon_1^- ) &= - \sqrt{2} \frac{
    \agl{1}{2} \sqr{2}{\tilde{\xi}}
    }{
    \sqr{\tilde{\xi}}{1}
    }
\end{aligned}
$$

end finally for $\epsilon_3^{(+)}$:
$$
\begin{aligned}
  \epsilon_3^{(+)} &= \frac{
    \tensor{{\lambda_1}}{_{\alpha}}
    \tensor{{\tilde{\lambda_3}}}{_{\dot{\alpha}}}
    }{
    \agl{1}{3}
    } \sqrt{2}\\
    \to 2\epsilon_2^- \epsilon_3^+ &= -(\sqrt{2})(\sqrt{2}) \frac{
    \agl{2}{1} \sqr{3}{\tilde{\xi}}
      }{
        \agl{1}{3} \sqr{\tilde{\xi}}{2}
      } \\
  &= -2 \frac{
    \agl{2}{1}
  }{
    \agl{1}{3}
  } \frac{
    \sqr{3}{\tilde{\xi} }
  }{
    \sqr{\tilde{\xi}}{2}
  }
\end{aligned}  
$$

Now we simplify:
$$
\begin{aligned}
  \frac{
    \agl{1}{2} \cancel{ \sqr{2}{\tilde{\xi}}}
    }{
      \agl{\xi}{1}
    } \frac{
      \agl{2}{1} \sqr{3}{ \tilde{\xi}}
    }{
      \cancel{ \sqr{2}{\tilde{\xi}}}
    } &= - \frac{ \agl{1}{2}^2 }{ \agl{1}{3} }
    \frac{ \sqr{3}{\tilde{\xi}} }{ \sqr{1}{\tilde{\xi}} } \\
    &= \frac{ \sqr{3}{\tilde{\xi}} }{ \sqr{1}{\tilde{\xi}} }
      \frac{ \agl{1}{2}^2 }{ \agl{3}{1} }
\end{aligned}
$$

#WORKING_ON: 29th feb
