<!--
@import "/dissertation/assets/custom.md" 
-->

<!-- #TODO: link to previous def that I have written  / Write definition of invariance -->

\begin{definition}[Invariance]

Take the following:


\begin{align}
  \lu{\alpha}\mud{\alpha} = \agl{\lambda}{\mu} &= \lu{\alpha}\muu{\beta}\tensor{\epsilon}{_{\alpha\beta}}\\
  \lmtd{\dot\alpha}\mtu{\alpha} &= \sqr{\lmt}{\tilde\mu}
\end{align}

Both of these are antisymmetric:

\begin{align}
  \sqr{\lmt}{\tilde\mu} = \mtd{\alpha}\ltu{\alpha} &= \epsilon_{\dot{\alpha}\dot{\beta}}\mtu{\beta}\lu{\dot\alpha}\\
  &= \mtu{\beta}(-\epsilon_{\dot{\beta}\dot{\alpha}} \ltu)\\
  &= -\ltd{\beta}\mtu{\beta}
\end{align}

Where \(\lambda, \lmt\) are two types of spinors:

\begin{align}
  \qq{Undotted:}& \lu{\alpha},   \ld{\alpha}\\
  \qq{Dotted:}& \mu_{\dot\alpha}, \mu^{\dot\alpha}
\end{align}
\end{definition}

## Dot product:


\begin{definition}[Dot Product]

In order to do a dot product using this convention:

\begin{align}
  \tensor{{p_1}}{^{\dot{\alpha}\alpha}} \tensor{{p_2}}{_{\dot{\alpha}\alpha}}
    &= \tensor{{\tilde{\lambda_1}}}{^{\dot{\alpha}}}
    \tensor{{\lambda_1}}{^\alpha}
    \tensor{{\lambda_2}}{_\alpha}
    \tensor{{\tilde{\lambda_2}}}{_{\dot{\alpha}}} \\
  &= \agl{1}{2} \sqr{2}{1} = 2(p_1p_2)
\end{align}

and

\[
  \begin{aligned}
    \agl{1}{2} &\equiv \tensor{{\lambda_1}}{^\alpha} \tensor{{\lambda_2}}{_\alpha}\\
    \sqr{1}{2} &\equiv \tensor{{\lambda_1}}{_{\dot{\alpha}}} \tensor{{\lambda_2}}{^{\dot{\alpha}}}
  \end{aligned} \qquad
  \begin{aligned}
    \lu{\alpha} &= \epsilon^{\alpha\beta}\ld{\beta} \\
    \ld{\alpha} &= \epsilon_{\alpha\beta}\lu{\beta} \\
  \end{aligned}
\]

Hence we define:

\begin{align}
  \lu{\alpha} &= \epsilon^{\alpha\beta}\ld{\beta}\\
  \ld{\alpha} &= \epsilon_{\alpha\beta}\lu{\beta}
\end{align}

Similar to dotted spinors:

\begin{align}
  \tensor{{\sigma_\mu}}{_{\alpha\dot{\alpha}}} &\equiv
    \left( \one, \vec{\sigma} \right)_{\alpha\dot{\alpha}}\\
  \tensor{{\sigma_\mu}}{^{\dot{\alpha}\alpha}} &\equiv
    \left( \one, \vec{\sigma} \right)^{\dot{\alpha}\alpha}
      \equiv \epsilon^{\alpha\beta}\epsilon_{\dot{\alpha}\dot{\beta}} \tensor{{\sigma_{\mu}}}{_{\beta\dot{\beta}}} \\
  \tensor{{\overline{\sigma}^{\mu}}}{^{\dot{\alpha}\alpha}} &\equiv
    \left( \one, -\vec{\sigma} \right)^{\dot{\alpha} \alpha} 
      \equiv \epsilon^{\alpha \beta}\epsilon^{\dot{\alpha}\dot{\beta}}\tensor{{\sigma_\mu}}{_{\beta \dot{\beta}}}
\end{align}

\end{definition}


<!-- #TODO: write definition for spinnors -->

<!-- #UPTO: 14th april 10:52  -->

 <!--
    - - Looking at gluons as particles
    - - massless
    - - spin 1
    - - two states of polarisation: helicity \(h=\pm 1\)
    -->

\begin{definition}[Polarisation vector]

 - \(\vec{k} =\) Momentum vector
 - \(\vec{\epsilon} =\) a Polarisation vector


Orthogonal such that \(\vec{\epsilon} ( \vec{k} ) \cdot \vec{k}=0\)

\begin{figure}
  \centering
  \begin{tikzpicture}[]
    \coordinate (origin) at (0,0);
    \coordinate (x) at (0,1);
    \coordinate (y) at (1,0);
    \coordinate (z) at ({0.7*cos(210)} ,{0.7*sin(210)} );
    \draw[->] (origin) -- (x) node[anchor=south] {\(\vec{k}\)};
    \draw[->] (origin) -- (y) node[anchor=west] {\(\vec{\epsilon}^{\small -}\)};
    \draw[->] (origin) -- (z) node[anchor=north east] {\(\vec{\epsilon}^{\small +}\)};
  \end{tikzpicture}
\end{figure}

\begin{align}
  \vec{k} &= \abs{\vec{k}} (0,0,1)\\
  \epsilon_L &= \frac{1}{\sqrt{2}}(1,i,0)\\
  \epsilon_L &= \frac{1}{\sqrt{2}}(1,-i,0)
\end{align}

In 4D:

\begin{align}
  \epsilon^\mu(\vec{k}^{\pm})
\end{align}

Because \(\mu\) index is better to represent in \(\alpha\dot{\alpha}\) form:

\begin{align}
  \epsilon^{(+)}_{\alpha\dot{\alpha}}(k) &= \sqrt{2} (\text{something } B)\\
  \epsilon^{(-)}_{\alpha\dot{\alpha}}(k) &= \sqrt{2} (\text{something } A)
\end{align}

Here we need to introduce the reference spinor (\(\mu\tilde{\mu}\)), such that:

\begin{align}
  \tilde\mu \not\parallel \tilde\lambda: \qquad
    (A)&=&\frac{\ld{\alpha}\mtd{\alpha}}{\sqr{\tilde\lambda}{\tilde\mu}} \\
  \mu \not\parallel \lambda: \qquad
    (B)&=&\frac{\lmtd{\dot{\alpha}}\mud{\alpha}}{\agl{\lambda}{\mu}}
\end{align}

We don't want denominator to vanish such that \(\frac{\#}{\agl{\lambda}{\lambda}\to 0}\), as this would cause it to divide by zero.

So we will use:

\begin{equation}
\mud{\alpha} \to \mu^{'} = a \mu_\alpha + b \lambda_\alpha
\end{equation}

Therefore we choose \(\epsilon^{(+)}_{\alpha\dot{\alpha}}\) leaving us with:

\begin{align}
  \epsilon^{(+)}_{\alpha\dot{\alpha}} - \frac{
    \ltd{\alpha} ( a \mu_\alpha + b \lambda_\alpha )
  }{
    a \agl{\lambda}{\mu} + \cancel{b \agl{\lambda}{\lambda}}
  }
\end{align}

Where this is a gauge freedom:

\begin{equation}
  \epsilon^{(+)}_{\alpha\dot{\alpha}}  + \# \ld{\alpha} \lmtd{\dot{\alpha}} = \epsilon
\end{equation}

\end{definition}

## Maxwell relations

How does this relate to Maxwell equations:

\begin{align}
  \vec{\nabla} \cdot \vec{\vec{E}} &= \rho &  \vec{\nabla}\cdot\vec{B} &=0 \\
  \vec{\nabla}\times \vec{E} &= -\pdv{\vec{B}}{t} & \vec{\nabla}\times \vec{B}&=\vec{J}+\pdv{\vec{E}}{t}
\end{align}

Taking a closer look at \(\vec{\nabla}\cdot\vec{B} =0\), we can set:

\begin{equation}
  B = \left(  \vec{\nabla} \times A\right)
\end{equation}

Then it follows that

\begin{equation}
  \vec{\nabla}\times \left( E+ \pdv{\vec{A}}{t} \right) = \vec{0}
\end{equation}

Examining this in abstract terms:

\begin{align}
  \partial_\mu F^{\mu\nu} &= J^\nu\\
  F^{\mu\nu} &= \partial^\mu A^\nu
\end{align}

There is a symmetry in gauge invariance.

\begin{align}
  \vec{B} &= \vec{\nabla}A & E &= -\vec{\nabla}A^0 - \pdv{\vec{A}}{t}
\end{align}

Leading to our definition:

\begin{equation}
  A^\mu \equiv \left( A^0, \vec{A} \right)
\end{equation}

References:
[@Plefka:2014aa pp. 17-18, eqs 1.78, 1.79]


Using

\begin{align}
  \vec{A}\times (\vec{B}\times \vec{C}) &= \vec{B}(\vec{A}\cdot\vec{C}) - \vec{C} (\vec{A}\cdot \vec{B})\\
  (a\times b) = \epsilon^{ijk}a^j b^k
\end{align}

Where \(\epsilon^{ijk}\) is the cross product / Levi Civita symbol.

Combing the above mentioned expansions, we will now find a different way to write the Maxwell equations:

### A new method of deriving \(J, \rho\) and \(F\)

\begin{align}
  \vec{\nabla}(\underbrace{\vec{\nabla}\times A}_{=\vec{B}}) &= J \pdv{t}(\underbrace{-\vec{\nabla}A^0 - \pdv{\vec{A}}{t} }_{=E})\\
  &= \vec{\nabla}(\vec{\nabla}\cdot\vec{A}) - \vec{\nabla}^2\vec{A}\\
  &= \vec{\nabla}(\vec{\nabla}\cdot\vec{A}) - \vec{\nabla}^2\vec{A}\\
  &= \left( \pdv[2]{t} - \vec{\nabla}^2 \right)\vec{A} +\vec{\nabla}\left(\vec{\nabla}\cdot\vec{A}+ \pdv{A^0}{t}  \right) = \vec{J}
\end{align}

\begin{align}
  \vec{\nabla}\cdot\left(- \vec{\nabla}\cdot\vec{A}- \pdv{A}{t} \right) &= \rho\\
  \left( \pdv[2]{t} - \vec{\nabla}^2 \right)A^0 - \pdv{t} \left( \vec{\nabla}\cdot \vec{A} + \pdv{A^0}{t} \right) &= \rho
\end{align}

This leads us to a new operator '\(\Box\)' for a four-vector, defined as:

\begin{equation}
  \Box A^\mu = \partial^\mu \left( \partial_\nu A^\nu \right) = J^\mu
\end{equation}

Where we use:

  - a \(F^{\mu\nu} = \partial^\mu A^\nu - \partial^\nu A^\mu\)
  - a \(\partial_\mu F^{\mu\nu} = J^\nu\)

\begin{definition}[Gauge redundancy]

\begin{align}
  A^\mu &\to A^\mu + \partial^\mu \Lambda\\
  F^{\mu\nu}&\to F_{\mu\nu}
\end{align}

\end{definition}

