<!--
@import "/dissertation/assets/custom.md"
 -->

## Contraction using \(\left[ \quad  \right]\) and \(\langle \quad \rangle\) notation

 In order to move back and forth between our

 \begin{align}
   \agl{\lambda}{\chi} &\equiv& \lambda^\alpha \chi^\beta \epsilon_{\alpha\beta} &= \lambda^\alpha \chi_\alpha
   \\
   \ltd{\alpha}\tilde{\chi}^{\dot{\alpha}} &=& \epsilon_{\dot{\alpha}\beta}\ltu{\beta}\ltu{\alpha} &\equiv \sqr{\tilde{\lambda}}{\tilde{\chi}}
   \\
   2(p_i\cdot p_j) &\equiv& \tensor{{p_i}}{_{\alpha\dot{\alpha}}} \tensor{{p_i}}{^{\dot{\alpha}\alpha}} &= \agl{i}{j} \sqr{j}{i}
 \end{align}

\begin{definition}[Box operator]

\begin{equation}
  \Box \equiv \partial_\mu \partial^\mu \equiv \partial_0 \partial^0 +\partial_i \partial^i = \partial_j^2 - \nabla^2
  \label{eq:box_operator}
\end{equation}

\end{definition}

It has the following properties:

*   For massless particles: \(\left( \Box + m^2 \right) \phi = 0\)
*   Transform for \(\partial_\mu: \partial_\mu e^{ikx}\) for massless particles (i.e. where  \(k^2 = m^2\)):

### Weyl Spinors and equations

\begin{definition}[Weyl Equations]

\begin{align}
  i\partial_\mu \tensor{{\bar{\sigma}}}{^{\dot{\alpha}\alpha}} \Psi_{\alpha} = 0\\
  i\partial_\mu \tensor{\sigma}{_{\alpha \dot{\alpha}}} \tilde{\Psi}_{\alpha} = 0
\end{align}

Where \(\Psi_\alpha, \tilde{\Psi}_\alpha\) are Weyl spinors
\end{definition}

What do we need to solve \(\Psi_\alpha = \xi_\alpha e^{ikx}\):

\begin{align}
  i\partial^{\dot{\alpha}\alpha} \left( \xi_\alpha e^{ikx}\right) &= i^2 k^{\dot{\alpha}\alpha}\xi_\alpha e^{ikx} \\
  &= -\lu{\alpha} \ltu{\alpha} \xi_\alpha e^{ikx}
\end{align}

\begin{definition}[Spin operator \(\hat{h}\)]

\begin{equation}
  \hat{h} = -\frac{1}{2}\lambda \pdv{\lambda} + \frac{1}{2} \pdv{\tilde{\lambda}} \tilde{\lambda}
\end{equation}

\end{definition}

## Creating Amplitudes for a three particle interaction:

\begin{figure}  
  \centering
  \input{assets/amplitude_3pointsimple.tex}
  \caption{Feynman diagram of a three particle interaction}
\end{figure}


\begin{equation}
  A(1,2,3) \approx \agl{1}{2} \agl{2}{3} \agl{3}{1}
\end{equation}

Mixing brackets for three particles doesn't work, for example a three particle "Scattering":

\begin{align}
  \agl{1}{2} \sqr{2}{3} \agl{3}{1} &to p_1 + p_2 + p_3 = 0\\
  &\to p_1 = -(p_2 + p_3)
\end{align}

As we are looking at massless particles; here our equation goes:

\begin{align}
  p_1^2 &= 0\\
  & = p_2^2 + p_3^2 + 2(p_2 \cdot p_3)\\
  &= 2(p_2 \cdot p_3)\\
  \implies p_1 \cdot p_2 &= p_2 \cdot p_3 = p_3 \cdot p_1  = 0
\end{align}

And complex momenta:

\begin{align}
  2p_1 \cdot p_2 &= 2p_2 \cdot p_3 = 2p_3 \cdot p_1 \\
  \implies \agl{1}{2} \sqr{2}{1} &= 0\\
  \agl{2}{3} \sqr{3}{1} &= 0\\
  \agl{3}{1} \sqr{1}{3} &= 0\\
\end{align}

[@Plefka:2014aa, pp 17, section 1.11 Vanishing Tree Amplitudes]

We will use this and the following to explore a complex momenta:

\begin{align}
\qq{When} \agl{1}{2} &= 0
   \ld{1} &\parallel \ld{2}\\
   \tensor{{\ld{1}}}{_{\alpha}} &= a \tensor{{\ld{2}}}{_{\alpha}}\\
   A(1,2,3) &= \begin{cases} \overbrace{\agl{1}{2}}^{a_1} \overbrace{\agl{2}{3}}^{a_2} \overbrace{\agl{3}{1}}^{a_3}\\
     \underbrace{\sqr{1}{2}}_{\tilde{a_1}}
     \underbrace{\sqr{2}{3}}_{\tilde{a_3}}
     \underbrace{\sqr{3}{1}}_{\tilde{a_3}}
   \end{cases}
\end{align}


## Examples
### Simple using \(\sqr{\quad}{\ }\):

\begin{align}
  \frac{
    \sqr{1}{2}^3
    }{
    \sqr{2}{3} \sqr{3}{1}
    } &=
     &1: + \frac{1}{2}(3-1) &= +1\\
    &&2: + \frac{1}{2}(3-1) &= +1\\
    &&3: + \frac{1}{2}(0-2) &= -1\\
\end{align}

### Simple using \(\agl{\quad}{ }\):

\begin{align}
  \frac{
    \agl{1}{2}^3
    }{
    \agl{2}{3} \agl{3}{1}
    } &=
     &1: - \frac{1}{2}(3-1) &= -1\\
    &&2: - \frac{1}{2}(3-1) &= -1\\
    &&3: - \frac{1}{2}(0-2) &= +1\\
\end{align}

Note:

\begin{align}
  \agl{i}{j} &= - \frac{1}{2}(\qq{\(U_i\)} - \qq{\(D_j\)} )\\
  \sqr{i}{j} &= + \frac{1}{2}(\qq{\(U_i\)} - \qq{\(D_j\)} )
\end{align}


<!--
   - MHV examples:
   - a
   -->
