Why $x_{\dot{\alpha}\alpha}$? What is this object?

For the Lorenz transformation $P^\mu \to \tensor{\Lambda}{^\mu_\nu} \rho^\nu \equiv \rho^{\prime \nu}$:
$$
\begin{aligned}
  P_{\alpha \dot{\alpha}} &= x \rho^{\mu}\sigma_{\mu \alpha \dot{\alpha}}\\
  &= MpM^\dagger
\end{aligned}
$$

Using $P^mu\rho_\mu = \det{p}$, the following can be obtained:
$$
\begin{aligned}
  \det{MpM^\dagger} &= \det{p}\\
  \det{M}\det{p}\det{M^\dagger} &= \det{p}\\
  \det{M} &= 1
\end{aligned}
$$

Expanding on this, the can arrive at the following explanation:
$$
  P_{\alpha \dot{\alpha}} = \ld{\alpha}\ld{\dot{\alpha}} = \begin{pmatrix}
    \rho^0 +\rho^3 & \rho^1 - i\rho^2\\
    \rho^1 + i\rho^2 & \rho^0 - \rho^2
\end{pmatrix},
  \rho^0 = \rho_{1\dot{1}}
$$

This makes the ($\lambda_{\alpha \dot{\alpha}}$) an operation.

$$
  \underbrace{SO(1,3)}_{\qq{group}} \to \underbrace{SL(2, \CC)\times SL(2,\CC)}_{\qq{group} \mathbb{Z_2}}
$$

A transformation is a representation of this group; **Spinors**:

\begin{definition}[Spinor Group]
The spinor group is a transformation as follows:
$$
\begin{aligned}
  \tensor{\Psi}{^{\prime}_\alpha} &= \tensor{M}{_\alpha^\beta}\tensor{\Psi}{_\beta}\\
  \tensor{\bar{\Psi}}{^{\prime}_{\dot{\alpha}}} &= \tensor{M}{_{\dot{\alpha}}^{\dot{\beta}}}\tensor{\bar{\Psi}}{_\beta}\\
\end{aligned}
$$

Such that $\tensor{M}{^0_0}$ belongs to $SL(2,\CC)$, with $\det{M}=\one$
\end{definition}

The object which do not transform under $\tensor{\Psi}{^{\prime}_\alpha}, \tensor{\bar{\Psi}}{^{\prime}_{\dot{\alpha}}}$ build the objects which are invariant under Lorenz group.

# Levi Cevita symbol:

$$ \epsilon_{\alpha \beta} = \begin{pmatrix} 0 & 1 \\ -1 & 0 \end{pmatrix} $$

How does this transform with $M$

$$
  \epsilon_{\alpha\beta} \to \\
  \tensor{M}{_\alpha^{\alpha^{\prime}}} \\
  \tensor{M}{_\beta^{\beta^{\prime}}}\\
  \epsilon_{\alpha^{\prime} \beta^{\prime}}
$$

And this is precisely $\epsilon_{\alpha\beta} \det{M} = \epsilon_{\alpha\beta}$ and therefore invariant.


\begin{definition}[Spinors]
$$
\begin{aligned}
  \ld{\alpha} &= \epsilon_{\alpha\beta} \lu{\beta} &
  \lu{\alpha} &\equiv \epsilon^{\alpha\beta} \ld{\beta} \\
  \lmtd{\dot\alpha} &= \epsilon_{\dot{\alpha}\dot{\beta}} \ltu{\beta} &
  \ltu{\alpha} &\equiv \epsilon^{\dot{\alpha}\dot{\beta}} \lmtd{\dot\beta}
\end{aligned}
$$
\end{definition}

Proof:
$$
\begin{aligned}
  \lu{\alpha\prime} &= \epsilon^{\alpha\beta}\tensor{M}{_\beta^\gamma}\ld{\gamma}\\
  &= \underbrace{\epsilon^{\alpha\beta} \tensor{M}{_\beta^\gamma}}_{ \tensor{\left [ \left( M^T \right)^{-1} \right ]}{^{\alpha}_{\delta}} \lu{\delta}} \epsilon_{\gamma\delta} \lu{\delta}\\
  \to \lu{\alpha'} &= \lu{\delta} \tensor{\left( M^{-1} \right)}{_{\delta} ^{\alpha}}\\
  \tensor{\epsilon}{^{\alpha\beta}}\tensor{M}{_\beta^\gamma}\tensor{\epsilon}{_{\gamma\delta}} &\eqq \tensor{ \left( M^{-1} \right) }{_\delta^\alpha}
\end{aligned}
$$

*Side note* about $\epsilon\sigma^\mu\epsilon$, where:
$$
\begin{aligned}
  \epsilon =& \begin{pmatrix}0 & -1 \\ 1 & 0\end{pmatrix} =& -i\sigma_2\\
  \epsilon =& \begin{pmatrix}0 & 1 \\ -1 & 0\end{pmatrix} =& i\sigma_2\\
  \sigma_2 =& \begin{pmatrix}0 & -i \\ i & 0\end{pmatrix}
\end{aligned}
$$

\begin{definition}[$\det$]
$$
\tensor{\epsilon}{^{\alpha\beta}} \tensor{\epsilon}{_{\beta\rho}} \equiv \tensor{\delta}{^\alpha_\rho}
$$

\end{definition}
