<!--
@import "/dissertation/assets/custom.md"
 -->

## Deriving simplest 4-point MHV amplitude

Starting from a negative helicity amplitude, with a result of
$$A_{MHV}(1^- 2^- 3^+ 4^+) = \frac{\ag{12}^4}{\ag{12}\ag{23}\ag{34}\ag{41}}$$

### Special shifted:
$$
Case [1]
\left \{
\begin{aligned}
  \hat \lambda_4 &= \lambda_4 - z \lambda_1\\
  \hat{\tilde{\lambda}}_1 &= \tilde{\lambda}_1 + z\tilde{\lambda}_4
\end{aligned}
\right \}
=\bas{4}{1}
$$

For this, it can be easily seen that the poles come from $\ag{34}$

$$
\begin{aligned}
  \ag{\hat 4 1} &= \ag{41} - \cancelto{0}{ z\ag{11} }\\
  &= \ag{41}
\end{aligned}  
$$

Of the $\overline{MHV}$ and

\begin{figure}

\begin{subfigure}[t]{.5\linewidth}
  \centering
  \input{assets/mhv_4particle3.tex}
  \caption{$\overline{MHV}$  amplitude goes to zero, does not exist, as all LHS are + and all RHS are -}\label{fig:mhv_4particle3}
\end{subfigure}
\begin{subfigure}[t]{.5\linewidth}
  \centering
  \input{assets/mhv_4particle3_alt.tex}
  \caption{$MHV$ amplitude }\label{fig:mhv_4particle3_alt}
\end{subfigure}
\caption{$MHV$ amplitude calculations. One of these must go to zero, as there will only be one pole}
\end{figure}

The From the two amplitudes above ( $\overline{MHV}$  fig \ref{fig:mhv_4particle3} , and $MHV$ fig \ref{fig:mhv_4particle3_alt})). We can immediately see that using the combinations of $+$ and $-$ on $A_L$ and $A_R$; only one of the objects is physically possible. We will now use this to calculate the position of the pole from the $MHV$ amplitude:

$$
\begin{aligned}
  z_p &= (p_3 + \hat{p}_4 (z_p))^2\\
  &= 0\\
  &= \ag{3 \hat{4}} \sq{\hat{4} 3}\\
  &= \ag{3 \hat{4}} \sq{4 3} & \qq{NB no hat}\\
  &= 0\\
  &\implies \ag{34} - z\ag{31} = 0\\
  \therefore & z_p = \frac{\ag{34}}{\ag{31}} & \qq{pole}
\end{aligned}
$$

This is an important finding, and shows that momentum $\hat p$, will not generally be on-shell, but using this method, it keeps it on-shell.

### $\hat{p}$:
$$
\begin{aligned}
  A_R &= \frac{\ag{12}^3}{\ag{2 \hat{p} } \ag{\hat p 1}} &= \frac{\ag{12}^2}{\ag{2\hat p} \ag{\hat p 1}}\\
  A_L &= \frac{\sq{3 \hat 4}^3}{\sq{\hat 4 \hat p} \sq{\hat p 3}} &= \frac{\sq{34}^3}{\sq{4 \hat p} \sq{\hat p 3}}
\end{aligned}
$$

$$
  \frac{i}{(p_3 + p_4)^2} = \frac{\ag{12}^3}{\ag{2 \hat p}\ag{\hat p 1}} \cdot \frac{i}{\ag{34}\sq{43}} \cdot \frac{\sq{34}^3}{\sq{4 \hat p} \sq{\hat p 3}}
$$

For this, we have a possible pairing:
$$
\begin{aligned}
  \ag{\hat p 1} \sq{4 \hat p} &= \sq{4 \hat p}\sq{\hat p 1}\\
  &= \bsma{4}{\hat p}{1}\\
\end{aligned}
$$

Here we are looking for a way to keep out particles on shell, so we use the complex momentum, and find the correct particles momentum to work allow for this calculation. In this case, we are choosing $\hat p = \hat{\lambda}_1 + z\lambda_2$:

$$
\begin{aligned}
  &= \bsma{4}{\hat 1 + 2}{1}\\
  &= \bsma{4}{1 + 2}{1} = \overbrace{ \cancelto{0}{ \bsma{4}{1}{1} } }^{ \quad\text{Using }\sq{41}\ag{11} = 0 } + \bsma{4}{2}{1}\\
  \bsma{4}{2}{1} &= \sq{42}\ag{21}
\end{aligned}
$$

What do we need? What are the spinors $\lambda_p$ and $\tilde{\lambda}_p$. We will change to a more systematic method of computation.

Only for the value of $z_p$ should we keep the masses on shell.

$$
  \hat p = \hat 1 + 2 = \lambda_p\tilde{\lambda}_p
$$

### $\hat{1}$:

$$
  \hat 1 + 2 = \lambda_1 (\underbrace{\tilde{\lambda}_1 + z_p \tilde{\lambda}_4}_{\substack{\text{Need to compute this.}\\ \text{Does it look like } \lambda \tilde{\lambda} ?} }) + \lambda_2 \tilde{\lambda}_2
$$

$$
\begin{aligned}
  \tilde{\lambda}_1 + z_p \tilde{\lambda}_4 &= \tilde{\lambda}_1 + \frac{\ag{34}}{\ag{31}} \tilde{\lambda}_4\\
  &= \frac{\overbrace{\ag{31}\tilde{\lambda}_1}^{3} + \overbrace{\ag{34}\tilde{\lambda}_4}^{4}}{\ag{31}}\\
  &= \frac{
    \bra{3} (
      \overbrace{ p_1 + p+4}^{
        \substack{\text{Can look at}\\ \text{contributions from}\\ \text{other leg} }}
      )
      }{
        \ag{31}
      }
\end{aligned}
$$

The momentum of each particle can also be seen as a sum from all the other contributing particles momenta. In this way we are able to write our legs in a different form: $p_1 + p_4 = -p_2 -p_3$. And so continuing with this we substitute it back into the form we arrived at above:

$$
\begin{aligned}
  (\tilde{\lambda}_1 + z_p \tilde{\lambda}_4 ) &= -\frac{\bra{3}(2+3)}{\ag{31}}\\
  &= \frac{-\ag{32}\tilde{\lambda}_2}{\ag{31}}
\end{aligned}
$$

$\hat p$ in a factorised form:

$$
\begin{aligned}
  \hat p &= -\frac{\ag{32}}{\ag{31}}\lambda_1\tilde{\lambda}_2 +\lambda_2\tilde{\lambda}_2\\
  &= -\frac{\ag{32}}{\ag{31}}(\lambda_1 +\lambda_2)\tilde{\lambda}_2\\
  \ag{\hat p 1} &= \ag{21} \\
  \ag{2 \hat p} &= \underbrace{-\ag{21}}_{=\ag{12}} \frac{\ag{32}}{\ag{31}}
\end{aligned}
$$

This leaves us with the following:
$$
\begin{aligned}
  \sq{4 \hat p} &= \sq{42} \\
  \sq{\hat p 3} &= \sq{23}
\end{aligned}
$$

Now putting everything together:

$$
  \frac{
    \overbrace{\sq{34}^{\cancelto{2}{3}}}^{-} \overbrace{\ag{12}^{\cancelto{1}{3}}}^{-}
    }{
      \ag{34} \underbrace{\cancel{\sq{43}}}_{-} \sq{42} \sq{23} \cancel{\ag{12}} \frac{\ag{32}}{\ag{31}} \cancel{\ag{21}}
    } = \frac{
      \ag{12} \sq{34}^2 \ag{31}
      }{
        \ag{34} \sq{42} \sq{23} \ag{32}
      }\\
$$

This can be further simplified into our shifted pole:

$$
  \bams{3}{4}{2} = \bams{3}{-1 - \cancelto{0}{2} - \cancelto{0}{3}}{2}
$$

Where we have used the face that $\cancelto{0}{-2-3}$ because: $\bams{3}{-2}{2} = 0$

$$
  \bams{3}{-1}{2} = -\ag{31} \sq{12}
$$

We then substitute this into the denominator to produce:

$$
  \frac{
    \ag{12} \sq{34}^2 \cancel{\ag{31}}
    }{
      -\cancel{\ag{31}}\sq{12}\sq{23}\ag{32}
    }
$$

We can then group in the the terms in the denominator:

$$
\begin{aligned}
  \sq{12} \ag{32} &= \sq{12}\ag{23} (-)\\
  &= \bsma{1}{2}{3}(-)\\
  &= \bsma{1}{-\cancel{1} - \cancel{3} -4}{3} (-)\\
  &= + \sq{14}\ag{43}
\end{aligned}
$$

Multiplying both sides by $\frac{\sq{34}}{\sq{34}}$

### TODO: What does this mean here??
$$
  \ag{32}\sq{34} z\text{ bottom}
$$

TODO: ??? above

$$
\begin{aligned}
  &= -\ag{23} \sq{34}\\
  &= (-)(-) \ag{21} \sq{14}\\
  &= \frac{
    \cancelto{-}{\ag{12}} \sq{34}^2 \cancel{\ag{34}}\sq{34}
    }{
      - \cancel{\ag{31}} \sq{12} \sq{23} \cancel{\ag{21}} \sq{14}
    }\\
  \text{Finally } &= \frac{
    \sq{34}^3
    }{
    \sq{12}\sq{23}\sq{41}
    }
\end{aligned}
$$

We can check this result in the other direction
$$
\begin{aligned}
  \frac{\sq{34}^{\cancelto{2}{3}}
  }{
  \cancel{\sq{12}} \sq{23} \sq{41}
  } \cdot \frac{
    \ag{23} \cancel{\ag{34}} \ag{41}
    }{
    \ag{12}^{\cancelto{2}{3}}
    } \overset{?}{=} \pm \one
\end{aligned}
$$

Now we pair up the legs with the momentum:
$$
\begin{aligned}
  \sq{34} \ag{34} &= -2(p_3 \cdot p_4)\\
  \sq{12} \ag{12} &= -2(p_1 \cdot p_2) = -(p_1 + p_2)^2\\
  \sq{12} \ag{12} &= \sq{34} \ag{34}\\
  \ag{23} \sq{34} &= -\ag{21} \sq{14} = -\ag{12} \sq{41}\\
  \sq{34} \ag{41} &= -\sq{32} \ag{21} = -\sq{23} \ag{12}
\end{aligned}
$$

Putting all this together:

$$
\begin{aligned}
  = \frac{
    \ag{12} \sq{41} \sq{23} \ag{12}
    }{
    \ag{12}^2 \sq{23} \sq{41}
    } = \pm \one
\end{aligned}
$$

## Meeting Notes:
Slide equations:
$$
\begin{aligned}
  p &= \lambda \tilde{\lambda}\\
  p_\mu \to p_{\alpha\dot{\alpha}} &= p_\mu \sigma^\mu\\
  \text{show } p_\mu p^\mu = 0\\
  p_{\alpha\dot{\alpha}} \equiv \lambda_\alpha \tilde{\lambda}_\alpha\\
  \det{(p_{\alpha\dot{\alpha}})} &= p^2
\end{aligned}  
$$
