## Angular Momentum properties:

$$
\begin{aligned}
  \vec{J} &= \vec{x} \times \vec{p}\\
  &= xp_y - yp_x\\
\end{aligned}
$$

Using the a commutator:
$$
  \commutator{J^1}{J^2} = \commutator{x^2p^3 - x^3p^2}{x^3p^1 - x^1p^3}
$$

(Only commutator with same index are non-zero)
$$
\begin{aligned}
  \commutator{J_i}{J_i} &= 0\\
  \commutator{J_i}{J_j} &\ne 0\\
\end{aligned}
$$

This leads to the formal relation of angular momentum:

\begin{equation}
  \label{eq:angmomentum_commutator}
  \commutator{J^i}{J^j} = i \hbar J^{ijk} \sigma^k J^k
\end{equation}

This related transformation and sum to Noethers theorem

## Noethers Theorem
