A working through the formalism to arrive at the relativistic formalisms for

Starting with the

understanding energy through the Lagrangian equation

## Lagrangian Mechanics

\begin{equation}
  \label{eq:Hamiltonian}
  \hat H = \frac{\vec{p}^2}{2m}+V(q) \\
\end{equation}

\begin{equation}
  \L = -m\sqrt{1-\dvec{x}^2} \\
\end{equation}

\begin{equation}
  \label{eq:lagrangian2}
  p \equiv \pdv{\L}{\dvec{x}} = \frac{m\dvec{x}}{\sqrt{1-\dvec{x}^2}}
\end{equation}

\begin{equation}
  \label{eq:the_label}
  V(q) = \frac{1}{2}mv^2\\
\end{equation}

For small velocities, where $\vec{x}\ll 1$, we can say:
\begin{equation}
  \label{eq:lagrange_smallapprox}
  \sqrt{1-\dvec{x}^2} \approx 1-\frac{\dvec{x}^2}{2} + \dots
\end{equation}

### The time evolution of the system

Where $\H = \H(\vec{q}, \vec{p},t)$

\begin{equation}
  \label{eq:lagrangian_timeevolutionp}
  \dv{\vec{p}}{t} = -\pdv{\H}{\vec{q}}
\end{equation}

\begin{equation}
  \label{eq:lagrangian_timeevolutionq}
  \dv{\vec{q}}{t} = +\pdv{\H}{\vec{p}}
\end{equation}

Thus leaving us with the following set of equations:

$\H = T+V$:

\begin{equation}
  \label{eq:hamiltonian_lagrangian_basic}
  \frac{p^2}{2m} + \frac{1}{2}mv^2
\end{equation}


\begin{equation}
  \label{eq:hamiltonian_lagrangian}
  \H = \sum_i{\dvec{q}^i\pdv{\L}{\dvec{q}^i} -\L} = \sum_i{\dvec{q}^ip_i-\L}
\end{equation}

where

$$
p_i = \pdv{\L}{\dvec{q}^i}
$$

leading to
$$
\begin{aligned}
  \H &= m\dvec{x}^2 - (-m\sqrt{1-\dvec{x}^2})\\
  &= \frac{m\dvec{x}}{\sqrt{1-\dvec{x}^2}}\dvec{x} +m\sqrt{1-\dvec{x}^2} \\
  &= \frac{m\dvec{x}+m-m\dvec{x}^2}{\sqrt{1-\dvec{x}^2}}
\end{aligned}
$$

### Einstein Equation

Where we arrive at Einsteins formula, when setting c = 1
\begin{equation}
  \label{eq:einstein}
  \H = E = \frac{m}{\sqrt{1-\dvec{x}^2}}
\end{equation}

This explains the principal of relatively according to Einsteins equations, and allows us to begin setting up the formalism for representing interactions which include relativistic properties.

## Principal of relativity

(Classical theory of fields, @Landau:1975aa )
Inertial reference frame in which a body moves in respect to and without any other force enacting on it, proceeds at constant velocity.


### Reference frames:

Two inertial reference frames are related by:

$$
  \Delta x = x-x'
$$

where $\dv{x}{t}=0 \to x$ and $x'$ have same property of inertiality.


### Intervals:

Event: described by the place where it occured and times

$$
\begin{aligned}
  e_1 &= [t,x,y,z]\\
  \text{worldline }&= [t\to t', f(x,y,z)-f'(x,y,z)]
\end{aligned}
$$

Invariance of speed of light

## Lorentz group

The lorentz group is defined as being:

### Associative:

 $$
   A(BC) = (AB)C
 $$

### Unitary:

There exists an object such that:

$$
  U\cdot U^{-1} = \one
$$

#### Invariance under transformation:

$$
\begin{aligned}
  x^\mu &= \left( x^0, -\vec{x} \right)\\
  x'^\mu &= \tensor{\Lambda}{^\mu_\nu}x^\nu
\end{aligned}
$$

#### Metric:

$$
  \tensor{\eta}{_{\mu\nu}} = \begin{pmatrix}
  1 & 0 & 0 & 0\\
  0 & -1 & 0 & 0\\
  0 & 0 & -1 & 0\\
  0 & 0 & 0 & -1
  \end{pmatrix}
$$

such that:
$$
  \tensor{\eta}{_{\mu\nu}}x^\nu = \left( x^0, -\vec{x} \right)
$$

with the important quantity in relativity:
$$
\begin{aligned}
  x^2 &= \vec{x}\cdot \vec{x}
  &= x^\mu x_\mu
\end{aligned}
$$

### Proper and Improper group

Leaving us with the definition of the Lorentz group:

The condition $\det(\Lambda) = \pm 1$ divides $\L$ into two disconnected components $\L\pm$ , called proper and improper Lorentz transformations.
\begin{equation}
  \label{eq:lorentzgroup}
  \Lambda^T \eta \Lambda = \eta
\end{equation}

or with indicies:
$$
  \tensor{\Lambda}{^\mu_\rho} \tensor{\eta}{_{\mu\nu}} \tensor{\Lambda}{^\nu_\sigma} = \eta_{\rho \sigma}
$$

Here we have the following types of groups

proper group:
\begin{equation}
  \label{eq:proper_group}
  \det(\Lambda) = +1
\end{equation}

and the improper group
\begin{equation}
  \label{eq:improper_group}
  \det(\Lambda) = -1
\end{equation}

>The condition $\det(\Lambda) = \pm 1$ divides $\L$ into two disconnected components $\L\pm$ , called proper and improper Lorentz transformations.

#### The Orthochronus group

>The condition $\sgn (\tensor{\Lambda}{_{00}}) = \pm 1$ divides $\L$ into two disconnected components, which one denotes $\L^\uparrow$ and $\L^\downarrow$, and are called orthochronus and non-orthochronous. (jaff)

>The fundamental Lorentz transformations which we study are the restricted Lorentz group $\L^\uparrow_+$. These are the Lorentz transformations that are both proper, $\det \Lambda = +1$, and orthochronous, $\Lambda_{00} \ge 1$. There are some elementary transformations in $\L$ that map one component into another, and which have special names:

 - The Unit transformation $\one: \Lambda^T \eta \Lambda = \eta$
 - The parity transformation $P : (x_0,\vec{x}) \mapsto (x_0,-\vec{x})$.
 <!-- - The time-reversal transformation $T : (x_0,\vec{x}) \mapsto (-x_0,\vec{x})$.
 - The space-time-inversion transformation $PT : (x_0,\vec{x}) \mapsto (-x_0,-\vec{x})$. -->


 The _proper group_ and _orthochronus group_: $\tensor{\Lambda}{^0_0}>1$

$$
\begin{aligned}
  \tensor{(\Lambda \tilde{\Lambda})}{^0_0} &= \tensor{\Lambda}{^0_\mu} \tensor{\tilde{\Lambda}}{^\mu_0}\\
  &= \tensor{\Lambda}{^0_0} \tensor{\tilde{\Lambda}}{^0_0} + \tensor{\Lambda}{^0_1} \tensor{\tilde{\Lambda}}{^1_0} \ge 1
\end{aligned}
$$

An example of this is the unit transformation:

$$
\begin{aligned}
  \one &= \begin{pmatrix}
    1 & 0 & 0 & 0\\
    0 & 1 & 0 & 0\\
    0 & 0 & 1 & 0\\
    0 & 0 & 0 & 1
  \end{pmatrix} \\
\Lambda^T \eta \Lambda &= \eta
\end{aligned}
$$

(Parity)
$$
  P(x^0, \vec{x}) \mapsto ()
$$

The conditions for our transformation:

$$
\begin{aligned}
  \Lambda^T \eta \Lambda &= \eta\\
  \begin{pmatrix}
    a & c\\ b & d
  \end{pmatrix} \begin{pmatrix}
    1 & 0 \\ 0 & -1
  \end{pmatrix} \begin{pmatrix}
    a & b \\ c & d
  \end{pmatrix} &= \begin{pmatrix}
    1 & 0 \\ 0 & -1
  \end{pmatrix}
\end{aligned}
$$

The conditions for $a, b, c$ & $d$:
$$
\begin{pmatrix}
  \cosh \theta & \sinh \theta \\ sinh \theta & \cosh \theta
\end{pmatrix} = \begin{pmatrix}
  \gamma & \gamma \beta \\ \gamma \beta & \gamma
\end{pmatrix}
$$

and must satisfy $R^TR = \one$:


$$
\begin{pmatrix}x_{00} & x_{10}\\x_{01} & x_{11}\end{pmatrix}
\begin{pmatrix} \eta_{00} & \eta_{01}\\\eta_{10} & \eta_{11} \end{pmatrix}
\begin{pmatrix} x_{00} & x_{01}\\x_{10} & x_{11} \end{pmatrix} =
\begin{pmatrix} \eta_{00} & \eta_{01}\\\eta_{10} & \eta_{11} \end{pmatrix}
$$

$$
=\left[
\begin{array}{c|c}
  \begin{aligned}
    x_{00} &\left(\eta_{00} x_{00} + \eta_{10} x_{10}\right) + \\
    x_{10} &\left(\eta_{01} x_{00} + \eta_{11} x_{10}\right)
  \end{aligned} & \begin{aligned}
    x_{01} &\left(\eta_{00} x_{00} + \eta_{10} x_{10}\right) + \\
    x_{11} &\left(\eta_{01} x_{00} + \eta_{11} x_{10}\right)
  \end{aligned} \\
  \hline
  \begin{aligned}
  x_{00} &\left(\eta_{00} x_{01} + \eta_{10} x_{11}\right) +\\
  x_{10} &\left(\eta_{01} x_{01} + \eta_{11} x_{11}\right) \
  \end{aligned} & \begin{aligned}
  x_{01} & \left(\eta_{00} x_{01} + \eta_{10} x_{11}\right) + \\
  x_{11} & \left(\eta_{01} x_{01} + \eta_{11} x_{11}\right)
\end{aligned}
\end{array} \right]
$$

### Transformations:

A velocity transformation
$$
\begin{aligned}
  \dv{x'^0}(x') &= v &\implies \dd x' &= \gamma(\dd x + \beta \dd x^0)\\
  & &\implies \dd x'^0 &= \gamma(\dd x^0 + \beta \dd x)\\
\end{aligned}
$$

For small velocities:

$$
\begin{aligned}
S &= -mc^2 \int \dd t \sqrt{1-\frac{\dvec{x}^2}{c^2}}\\
 &\simeq \frac{1- \dvec{x}^2 }{\left(2c^2\right)^2}
\end{aligned}
$$


Using $p^2 = m^2$:

$$
  E(\dvec{x}) = \frac{m}{\sqrt{1-\dvec{x}^2}} \to m+m\frac{\dvec{x}^2}{2}
$$


Claim:
$$
\begin{aligned}
  (E, \vec{p}) &= \qq{4-momentum}\\
  &= \qq{4-velocity}
\end{aligned}
$$

There exists these two values

$$
\begin{aligned}
  p^\mu &\to \tensor{\Lambda}{^\mu_\nu} p^\nu \\
  x^\mu &\to \tensor{\Lambda}{^\mu_\nu} x^\nu
\end{aligned}
$$

To prove that this quantity os a 4-vector:

$$
\begin{aligned}
  v^\mu &= \dv{x^\mu}{\tau} \to  \dv{x^\mu}{x} \\
  \dv{x^\mu}{t} \dv{t}{\tau} &= \dv{x}{t}
\end{aligned}
$$



Lagrangian using the following Taylor expansion:

$$
\begin{cases}
  \sqrt{1+\epsilon} &\sim 1+\frac{\epsilon}{2} \\
  \frac{1}{1+\epsilon} &\sim 1-\epsilon
\end{cases}
$$

Combined:
$$
  \frac{1}{\sqrt{1-\epsilon}} = 1+ \frac{\epsilon}{2}
$$


(Fundamentally we are alloking at massless particles, where $p^2 = m^2 = 0$)
